Refactor

prim_rec.lean
@@ -1,3 +1,5 @@
+import .fin_seq
+
 inductive prim_rec: nat -> Type
 | zero: prim_rec 0
 | succ: prim_rec 1
@@ -5,124 +7,66 @@ inductive prim_rec: nat -> Type
 | comp: forall {k m}, prim_rec k -> (fin k -> prim_rec m) -> prim_rec m
 | prec: forall {k}, prim_rec k -> prim_rec (k + 2) -> prim_rec (k + 1)
 
+namespace prim_rec
 
-def curry {k} (v: nat) (a: fin k -> nat): (fin (k + 1)) -> nat
-| ⟨val, is_lt⟩ :=
-  begin
-    cases val with val',
-    exact v, -- arg(0) = v
-    apply a,
-    existsi val',
-    apply nat.lt_of_succ_lt_succ,
-    exact is_lt,
-  end
-
-
-def uncurry {k} (a: fin (k + 1) -> nat): prod nat (fin k -> nat) :=
-begin
-  split,
-  exact a 0,
-  intro arg,
-  cases arg with val is_lt,
-  apply a,
-  split,
-  show val + 1 < k + 1,
-  apply nat.succ_lt_succ,
-  exact is_lt,
-end
-
-
-lemma curry_of_uncurry: forall {k} (a: fin (k + 1) -> nat),
-  a = let p := uncurry a in
-      curry p.fst p.snd :=
-begin
-  intros k a,
-  apply funext,
-  intro arg,
-  cases arg with val is_lt,
-  cases val with val',
-  reflexivity,
-    show a ⟨nat.succ val', is_lt⟩ =
-  curry ((uncurry a).fst) ((uncurry a).snd) ⟨val' + 1, is_lt⟩,
-  unfold curry,
-  reflexivity,
-end
-
-
-def prim_eval : forall {k}, prim_rec k -> (fin k -> nat) -> nat
+def eval : forall {k}, prim_rec k -> (fin k -> nat) -> nat
 | 0 prim_rec.zero _arg := 0
 | 1 prim_rec.succ arg := arg 0 + 1
 | m (prim_rec.proj idx) arg := arg idx
 | m (@prim_rec.comp k .(m) (f: prim_rec k) g) arg
-  := prim_eval f (fun i, prim_eval (g i) arg)
+  := eval f (fun i, eval (g i) arg)
 | .(_) (@prim_rec.prec k f g) arg :=
   let h :=
   fun (v: nat) (arg: fin k -> nat),
-  @nat.rec (fun _, nat) (prim_eval f arg)
-    (fun (v': nat) (prev: nat), prim_eval g (curry prev (curry v' arg))) v in
-  let ⟨x, y⟩ := uncurry arg in
+  @nat.rec (fun _, nat) (eval f arg)
+    (fun (v': nat) (prev: nat), eval g (fin_seq.push prev (fin_seq.push v' arg))) v in
+  let ⟨x, y⟩ := fin_seq.pop arg in
   h x y
 
+lemma zero.is_zero: eval zero fin_seq.empty = 0 :=
+begin
+  reflexivity,
+end
 
-lemma succ_succ : forall x, prim_eval prim_rec.succ (fun _, x) = x + 1 :=
+lemma succ.is_succ: forall x, eval prim_rec.succ (fun _, x) = x + 1 :=
 fun x,
 calc
-  prim_eval prim_rec.succ (fun _, x) = x + 1 : by unfold prim_eval; reflexivity
+  eval prim_rec.succ (fun _, x) = x + 1 : by unfold eval; reflexivity
 
+lemma uncurry_1: forall v: nat, fin_seq.pop (fun _: fin 1, v) = ⟨v, fin_seq.empty⟩ :=
+  fin_seq.pop_1
 
-lemma uncurry_1: forall v: nat, uncurry (fun _: fin 1, v) = ⟨v, fun _, 0⟩ :=
+lemma curry_at_0: forall k v (rest: fin k -> nat), fin_seq.push v rest 0 = v :=
 begin
-  intro v,
-  have h: forall x: fin 0 -> nat, x = (fun _, 0),
-  {
-    intros x,
-    apply funext,
-    intro fin0,
-    cases fin0 with val is_lt,
-    cases is_lt,
-  },
-  calc
-   uncurry (fun _: fin 1, v)
-     = (v, fun arg: fin 0, fin.cases_on arg (fun _ _, v)) :
-           by simp only [uncurry]
- ... = (v, fun _, 0) : by rw h (fun arg: fin 0, fin.cases_on arg (fun _ _, v))
+  apply fin_seq.push_at_0
 end
 
-
-
-lemma curry_at_0: forall k v (rest: fin k -> nat), curry v rest 0 = v :=
-begin
-  intros k v rest,
-  reflexivity,
-end
-
-
-lemma curry_at_succ: forall k v (rest: fin k -> nat) (i: fin k), curry v rest (fin.succ i) = rest i
+lemma curry_at_succ: forall k v (rest: fin k -> nat) (i: fin k), fin_seq.push v rest (fin.succ i) = rest i
   :=
 begin
-  intros k v rest i,
-  cases i with i is_lt,
-  reflexivity,
+  apply fin_seq.push_at_succ,
 end
 
 
-def prim_id: prim_rec 1 := prim_rec.prec prim_rec.zero
+def id: prim_rec 1 := prim_rec.prec prim_rec.zero
   (prim_rec.comp prim_rec.succ (fun _, prim_rec.proj 0))
 
 
-lemma prim_id_is_id : forall x, prim_eval prim_id (fun _, x) = x :=
+lemma id.is_id : forall x, eval id (fun _, x) = x :=
 begin
   intro x,
   induction x with x' ih,
   reflexivity,
-  show prim_eval prim_id
+  show eval id
       (fun _ : fin 1, x' + 1) =
     x' + 1,
   calc
-    prim_eval prim_id
+    eval id
       (fun _ : fin 1, x' + 1)
-    = prim_eval prim_id
+    = eval id
       (fun _ : fin 1, x') + 1 : by reflexivity
 ... = x' + 1 :
       by rw ih
 end
+
+end prim_rec
