fin_seq.lean
@@ -1,0 +1,102 @@
+def fin_seq k (t: Type) := fin k -> t
+
+namespace fin_seq
+
+def push {t k} (v: t) (a: fin_seq k t): fin_seq (k + 1) t
+| ⟨val, is_lt⟩ :=
+  begin
+    cases val with val',
+    exact v, -- arg(0) = v
+    apply a,
+    existsi val',
+    apply nat.lt_of_succ_lt_succ,
+    exact is_lt,
+  end
+
+def pop {t k} (a: fin_seq (k + 1) t): prod t (fin_seq k t) :=
+begin
+  split,
+  exact a 0,
+  intro arg,
+  cases arg with val is_lt,
+  apply a,
+  split,
+  show val + 1 < k + 1,
+  apply nat.succ_lt_succ,
+  exact is_lt,
+end
+
+def empty: fin_seq 0 nat := fun _, 0
+
+def singleton {t: Type} (v: t): fin_seq 1 t := fun _, v
+
+lemma push_of_pop: forall {t: Type} {k} (a: fin_seq (k + 1) t),
+  a = let p := pop a in
+      push p.fst p.snd :=
+begin
+  intros t k a,
+  apply funext,
+  intro arg,
+  cases arg with val is_lt,
+  cases val with val',
+  reflexivity,
+    show a ⟨nat.succ val', is_lt⟩ =
+  push ((pop a).fst) ((pop a).snd) ⟨val' + 1, is_lt⟩,
+  unfold push,
+  reflexivity,
+end
+
+lemma empty_is_unique: forall x: fin_seq 0 nat, x = empty :=
+begin
+  intros x,
+  apply funext,
+  intro fin0,
+  cases fin0 with val is_lt,
+  cases is_lt,  
+end
+
+lemma pop_of_push: forall {t k} (v: t) (a: fin_seq k t),
+  (v, a) = pop (push v a) :=
+begin
+  intros t k v a,
+  simp [pop],
+  have left: v = push v a 0,
+  {
+    reflexivity,
+  },
+  rw <- left,
+  apply congr_arg,
+  apply funext,
+  intro x,
+  cases x with val is_lt,
+  reflexivity,
+end
+
+lemma pop_1: forall v: nat, pop (singleton v) = ⟨v, empty⟩ :=
+begin
+  intro v,
+  simp [singleton],
+  simp [pop],
+  have : forall x: fin 0 -> nat, (v, x) = (v, empty),
+  {
+    intro x,
+    rw empty_is_unique x,
+  },
+  apply this,
+end
+
+lemma push_at_0: forall {t k} v (rest: fin_seq k t), fin_seq.push v rest 0 = v :=
+begin
+  intros t k v rest,
+  reflexivity,
+end
+
+lemma push_at_succ: forall {t k} v (rest: fin_seq k t) (i: fin k), push v rest (fin.succ i) = rest i
+  :=
+begin
+  intros t k v rest i,
+  cases i with i is_lt,
+  reflexivity,
+end
+
+end fin_seq
